Rename `iprod` into `ofe_fun`.

theories/algebra/cmra.v
@@ -1465,41 +1465,41 @@ Proof.
 Qed.
 
 (* Dependently-typed functions *)
-Section iprod_cmra.
+Section ofe_fun_cmra.
   Context `{Hfin : Finite A} {B : A → ucmraT}.
-  Implicit Types f g : iprod B.
+  Implicit Types f g : ofe_fun B.
 
-  Instance iprod_op : Op (iprod B) := λ f g x, f x ⋅ g x.
-  Instance iprod_pcore : PCore (iprod B) := λ f, Some (λ x, core (f x)).
-  Instance iprod_valid : Valid (iprod B) := λ f, ∀ x, ✓ f x.
-  Instance iprod_validN : ValidN (iprod B) := λ n f, ∀ x, ✓{n} f x.
+  Instance ofe_fun_op : Op (ofe_fun B) := λ f g x, f x ⋅ g x.
+  Instance ofe_fun_pcore : PCore (ofe_fun B) := λ f, Some (λ x, core (f x)).
+  Instance ofe_fun_valid : Valid (ofe_fun B) := λ f, ∀ x, ✓ f x.
+  Instance ofe_fun_validN : ValidN (ofe_fun B) := λ n f, ∀ x, ✓{n} f x.
 
-  Definition iprod_lookup_op f g x : (f ⋅ g) x = f x ⋅ g x := eq_refl.
-  Definition iprod_lookup_core f x : (core f) x = core (f x) := eq_refl.
+  Definition ofe_fun_lookup_op f g x : (f ⋅ g) x = f x ⋅ g x := eq_refl.
+  Definition ofe_fun_lookup_core f x : (core f) x = core (f x) := eq_refl.
 
-  Lemma iprod_included_spec (f g : iprod B) : f ≼ g ↔ ∀ x, f x ≼ g x.
+  Lemma ofe_fun_included_spec (f g : ofe_fun B) : f ≼ g ↔ ∀ x, f x ≼ g x.
   Proof using Hfin.
-    split; [by intros [h Hh] x; exists (h x); rewrite /op /iprod_op (Hh x)|].
+    split; [by intros [h Hh] x; exists (h x); rewrite /op /ofe_fun_op (Hh x)|].
     intros [h ?]%finite_choice. by exists h.
   Qed.
 
-  Lemma iprod_cmra_mixin : CmraMixin (iprod B).
+  Lemma ofe_fun_cmra_mixin : CmraMixin (ofe_fun B).
   Proof using Hfin.
     apply cmra_total_mixin.
     - eauto.
-    - by intros n f1 f2 f3 Hf x; rewrite iprod_lookup_op (Hf x).
-    - by intros n f1 f2 Hf x; rewrite iprod_lookup_core (Hf x).
+    - by intros n f1 f2 f3 Hf x; rewrite ofe_fun_lookup_op (Hf x).
+    - by intros n f1 f2 Hf x; rewrite ofe_fun_lookup_core (Hf x).
     - by intros n f1 f2 Hf ? x; rewrite -(Hf x).
     - intros g; split.
       + intros Hg n i; apply cmra_valid_validN, Hg.
       + intros Hg i; apply cmra_valid_validN=> n; apply Hg.
     - intros n f Hf x; apply cmra_validN_S, Hf.
-    - by intros f1 f2 f3 x; rewrite iprod_lookup_op assoc.
-    - by intros f1 f2 x; rewrite iprod_lookup_op comm.
-    - by intros f x; rewrite iprod_lookup_op iprod_lookup_core cmra_core_l.
-    - by intros f x; rewrite iprod_lookup_core cmra_core_idemp.
-    - intros f1 f2; rewrite !iprod_included_spec=> Hf x.
-      by rewrite iprod_lookup_core; apply cmra_core_mono, Hf.
+    - by intros f1 f2 f3 x; rewrite ofe_fun_lookup_op assoc.
+    - by intros f1 f2 x; rewrite ofe_fun_lookup_op comm.
+    - by intros f x; rewrite ofe_fun_lookup_op ofe_fun_lookup_core cmra_core_l.
+    - by intros f x; rewrite ofe_fun_lookup_core cmra_core_idemp.
+    - intros f1 f2; rewrite !ofe_fun_included_spec=> Hf x.
+      by rewrite ofe_fun_lookup_core; apply cmra_core_mono, Hf.
     - intros n f1 f2 Hf x; apply cmra_validN_op_l with (f2 x), Hf.
     - intros n f f1 f2 Hf Hf12.
       destruct (finite_choice (λ x (yy : B x * B x),
@@ -1509,57 +1509,57 @@ Section iprod_cmra.
         exists (y1,y2); eauto. }
       exists (λ x, gg x.1), (λ x, gg x.2). split_and!=> -?; naive_solver.
   Qed.
-  Canonical Structure iprodR := CmraT (iprod B) iprod_cmra_mixin.
+  Canonical Structure ofe_funR := CmraT (ofe_fun B) ofe_fun_cmra_mixin.
 
-  Instance iprod_unit : Unit (iprod B) := λ x, ε.
-  Definition iprod_lookup_empty x : ε x = ε := eq_refl.
+  Instance ofe_fun_unit : Unit (ofe_fun B) := λ x, ε.
+  Definition ofe_fun_lookup_empty x : ε x = ε := eq_refl.
 
-  Lemma iprod_ucmra_mixin : UcmraMixin (iprod B).
+  Lemma ofe_fun_ucmra_mixin : UcmraMixin (ofe_fun B).
   Proof.
     split.
     - intros x; apply ucmra_unit_valid.
-    - by intros f x; rewrite iprod_lookup_op left_id.
+    - by intros f x; rewrite ofe_fun_lookup_op left_id.
     - constructor=> x. apply core_id_core, _.
   Qed.
-  Canonical Structure iprodUR := UcmraT (iprod B) iprod_ucmra_mixin.
+  Canonical Structure ofe_funUR := UcmraT (ofe_fun B) ofe_fun_ucmra_mixin.
 
-  Global Instance iprod_unit_discrete :
-    (∀ i, Discrete (ε : B i)) → Discrete (ε : iprod B).
+  Global Instance ofe_fun_unit_discrete :
+    (∀ i, Discrete (ε : B i)) → Discrete (ε : ofe_fun B).
   Proof. intros ? f Hf x. by apply: discrete. Qed.
-End iprod_cmra.
+End ofe_fun_cmra.
 
-Arguments iprodR {_ _ _} _.
-Arguments iprodUR {_ _ _} _.
+Arguments ofe_funR {_ _ _} _.
+Arguments ofe_funUR {_ _ _} _.
 
-Instance iprod_map_cmra_morphism
+Instance ofe_fun_map_cmra_morphism
     `{Finite A} {B1 B2 : A → ucmraT} (f : ∀ x, B1 x → B2 x) :
-  (∀ x, CmraMorphism (f x)) → CmraMorphism (iprod_map f).
+  (∀ x, CmraMorphism (f x)) → CmraMorphism (ofe_fun_map f).
 Proof.
   split; first apply _.
-  - intros n g Hg x; rewrite /iprod_map; apply (cmra_morphism_validN (f _)), Hg.
+  - intros n g Hg x; rewrite /ofe_fun_map; apply (cmra_morphism_validN (f _)), Hg.
   - intros. apply Some_proper=>i. apply (cmra_morphism_core (f i)).
-  - intros g1 g2 i. by rewrite /iprod_map iprod_lookup_op cmra_morphism_op.
+  - intros g1 g2 i. by rewrite /ofe_fun_map ofe_fun_lookup_op cmra_morphism_op.
 Qed.
 
-Program Definition iprodURF `{Finite C} (F : C → urFunctor) : urFunctor := {|
-  urFunctor_car A B := iprodUR (λ c, urFunctor_car (F c) A B);
-  urFunctor_map A1 A2 B1 B2 fg := iprodC_map (λ c, urFunctor_map (F c) fg)
+Program Definition ofe_funURF `{Finite C} (F : C → urFunctor) : urFunctor := {|
+  urFunctor_car A B := ofe_funUR (λ c, urFunctor_car (F c) A B);
+  urFunctor_map A1 A2 B1 B2 fg := ofe_funC_map (λ c, urFunctor_map (F c) fg)
 |}.
 Next Obligation.
   intros C ?? F A1 A2 B1 B2 n ?? g.
-  by apply iprodC_map_ne=>?; apply urFunctor_ne.
+  by apply ofe_funC_map_ne=>?; apply urFunctor_ne.
 Qed.
 Next Obligation.
-  intros C ?? F A B g; simpl. rewrite -{2}(iprod_map_id g).
-  apply iprod_map_ext=> y; apply urFunctor_id.
+  intros C ?? F A B g; simpl. rewrite -{2}(ofe_fun_map_id g).
+  apply ofe_fun_map_ext=> y; apply urFunctor_id.
 Qed.
 Next Obligation.
-  intros C ?? F A1 A2 A3 B1 B2 B3 f1 f2 f1' f2' g. rewrite /=-iprod_map_compose.
-  apply iprod_map_ext=>y; apply urFunctor_compose.
+  intros C ?? F A1 A2 A3 B1 B2 B3 f1 f2 f1' f2' g. rewrite /=-ofe_fun_map_compose.
+  apply ofe_fun_map_ext=>y; apply urFunctor_compose.
 Qed.
-Instance iprodURF_contractive `{Finite C} (F : C → urFunctor) :
-  (∀ c, urFunctorContractive (F c)) → urFunctorContractive (iprodURF F).
+Instance ofe_funURF_contractive `{Finite C} (F : C → urFunctor) :
+  (∀ c, urFunctorContractive (F c)) → urFunctorContractive (ofe_funURF F).
 Proof.
   intros ? A1 A2 B1 B2 n ?? g.
-  by apply iprodC_map_ne=>c; apply urFunctor_contractive.
+  by apply ofe_funC_map_ne=>c; apply urFunctor_contractive.
 Qed.
