theories/algebra/ofe.v
@@ -1088,17 +1088,17 @@ Proof.
 Qed.
 
 (* Dependently-typed functions *)
-(* We make [iprod] a definition so that we can register it as a canonical
+(* We make [ofe_fun] a definition so that we can register it as a canonical
 structure. *)
-Definition iprod {A} (B : A → ofeT) := ∀ x : A, B x.
+Definition ofe_fun {A} (B : A → ofeT) := ∀ x : A, B x.
 
-Section iprod.
+Section ofe_fun.
   Context {A : Type} {B : A → ofeT}.
-  Implicit Types f g : iprod B.
+  Implicit Types f g : ofe_fun B.
 
-  Instance iprod_equiv : Equiv (iprod B) := λ f g, ∀ x, f x ≡ g x.
-  Instance iprod_dist : Dist (iprod B) := λ n f g, ∀ x, f x ≡{n}≡ g x.
-  Definition iprod_ofe_mixin : OfeMixin (iprod B).
+  Instance ofe_fun_equiv : Equiv (ofe_fun B) := λ f g, ∀ x, f x ≡ g x.
+  Instance ofe_fun_dist : Dist (ofe_fun B) := λ n f g, ∀ x, f x ≡{n}≡ g x.
+  Definition ofe_fun_ofe_mixin : OfeMixin (ofe_fun B).
   Proof.
     split.
     - intros f g; split; [intros Hfg n k; apply equiv_dist, Hfg|].
@@ -1109,18 +1109,18 @@ Section iprod.
       + by intros f g h ?? x; trans (g x).
     - by intros n f g ? x; apply dist_S.
   Qed.
-  Canonical Structure iprodC := OfeT (iprod B) iprod_ofe_mixin.
+  Canonical Structure ofe_funC := OfeT (ofe_fun B) ofe_fun_ofe_mixin.
 
-  Program Definition iprod_chain `(c : chain iprodC)
+  Program Definition ofe_fun_chain `(c : chain ofe_funC)
     (x : A) : chain (B x) := {| chain_car n := c n x |}.
   Next Obligation. intros c x n i ?. by apply (chain_cauchy c). Qed.
-  Global Program Instance iprod_cofe `{∀ x, Cofe (B x)} : Cofe iprodC :=
-    { compl c x := compl (iprod_chain c x) }.
-  Next Obligation. intros ? n c x. apply (conv_compl n (iprod_chain c x)). Qed.
+  Global Program Instance ofe_fun_cofe `{∀ x, Cofe (B x)} : Cofe ofe_funC :=
+    { compl c x := compl (ofe_fun_chain c x) }.
+  Next Obligation. intros ? n c x. apply (conv_compl n (ofe_fun_chain c x)). Qed.
 
-  Global Instance iprod_inhabited `{∀ x, Inhabited (B x)} : Inhabited iprodC :=
+  Global Instance ofe_fun_inhabited `{∀ x, Inhabited (B x)} : Inhabited ofe_funC :=
     populate (λ _, inhabitant).
-  Global Instance iprod_lookup_discrete `{EqDecision A} f x :
+  Global Instance ofe_fun_lookup_discrete `{EqDecision A} f x :
     Discrete f → Discrete (f x).
   Proof.
     intros Hf y ?.
@@ -1130,61 +1130,61 @@ Section iprod.
     unfold g. destruct (decide _) as [Hx|]; last done.
     by rewrite (proof_irrel Hx eq_refl).
   Qed.
-End iprod.
+End ofe_fun.
 
-Arguments iprodC {_} _.
+Arguments ofe_funC {_} _.
 Notation "A -c> B" :=
-  (@iprodC A (λ _, B)) (at level 99, B at level 200, right associativity).
+  (@ofe_funC A (λ _, B)) (at level 99, B at level 200, right associativity).
 
-Definition iprod_map {A} {B1 B2 : A → ofeT} (f : ∀ x, B1 x → B2 x)
-  (g : iprod B1) : iprod B2 := λ x, f _ (g x).
+Definition ofe_fun_map {A} {B1 B2 : A → ofeT} (f : ∀ x, B1 x → B2 x)
+  (g : ofe_fun B1) : ofe_fun B2 := λ x, f _ (g x).
 
-Lemma iprod_map_ext {A} {B1 B2 : A → ofeT} (f1 f2 : ∀ x, B1 x → B2 x)
-  (g : iprod B1) :
-  (∀ x, f1 x (g x) ≡ f2 x (g x)) → iprod_map f1 g ≡ iprod_map f2 g.
+Lemma ofe_fun_map_ext {A} {B1 B2 : A → ofeT} (f1 f2 : ∀ x, B1 x → B2 x)
+  (g : ofe_fun B1) :
+  (∀ x, f1 x (g x) ≡ f2 x (g x)) → ofe_fun_map f1 g ≡ ofe_fun_map f2 g.
 Proof. done. Qed.
-Lemma iprod_map_id {A} {B : A → ofeT} (g : iprod B) :
-  iprod_map (λ _, id) g = g.
+Lemma ofe_fun_map_id {A} {B : A → ofeT} (g : ofe_fun B) :
+  ofe_fun_map (λ _, id) g = g.
 Proof. done. Qed.
-Lemma iprod_map_compose {A} {B1 B2 B3 : A → ofeT}
-    (f1 : ∀ x, B1 x → B2 x) (f2 : ∀ x, B2 x → B3 x) (g : iprod B1) :
-  iprod_map (λ x, f2 x ∘ f1 x) g = iprod_map f2 (iprod_map f1 g).
+Lemma ofe_fun_map_compose {A} {B1 B2 B3 : A → ofeT}
+    (f1 : ∀ x, B1 x → B2 x) (f2 : ∀ x, B2 x → B3 x) (g : ofe_fun B1) :
+  ofe_fun_map (λ x, f2 x ∘ f1 x) g = ofe_fun_map f2 (ofe_fun_map f1 g).
 Proof. done. Qed.
 
-Instance iprod_map_ne {A} {B1 B2 : A → ofeT} (f : ∀ x, B1 x → B2 x) n :
+Instance ofe_fun_map_ne {A} {B1 B2 : A → ofeT} (f : ∀ x, B1 x → B2 x) n :
   (∀ x, Proper (dist n ==> dist n) (f x)) →
-  Proper (dist n ==> dist n) (iprod_map f).
-Proof. by intros ? y1 y2 Hy x; rewrite /iprod_map (Hy x). Qed.
+  Proper (dist n ==> dist n) (ofe_fun_map f).
+Proof. by intros ? y1 y2 Hy x; rewrite /ofe_fun_map (Hy x). Qed.
 
-Definition iprodC_map {A} {B1 B2 : A → ofeT} (f : iprod (λ x, B1 x -n> B2 x)) :
-  iprodC B1 -n> iprodC B2 := CofeMor (iprod_map f).
-Instance iprodC_map_ne {A} {B1 B2 : A → ofeT} :
-  NonExpansive (@iprodC_map A B1 B2).
+Definition ofe_funC_map {A} {B1 B2 : A → ofeT} (f : ofe_fun (λ x, B1 x -n> B2 x)) :
+  ofe_funC B1 -n> ofe_funC B2 := CofeMor (ofe_fun_map f).
+Instance ofe_funC_map_ne {A} {B1 B2 : A → ofeT} :
+  NonExpansive (@ofe_funC_map A B1 B2).
 Proof. intros n f1 f2 Hf g x; apply Hf. Qed.
 
-Program Definition iprodCF {C} (F : C → cFunctor) : cFunctor := {|
-  cFunctor_car A B := iprodC (λ c, cFunctor_car (F c) A B);
-  cFunctor_map A1 A2 B1 B2 fg := iprodC_map (λ c, cFunctor_map (F c) fg)
+Program Definition ofe_funCF {C} (F : C → cFunctor) : cFunctor := {|
+  cFunctor_car A B := ofe_funC (λ c, cFunctor_car (F c) A B);
+  cFunctor_map A1 A2 B1 B2 fg := ofe_funC_map (λ c, cFunctor_map (F c) fg)
 |}.
 Next Obligation.
-  intros C F A1 A2 B1 B2 n ?? g. by apply iprodC_map_ne=>?; apply cFunctor_ne.
+  intros C F A1 A2 B1 B2 n ?? g. by apply ofe_funC_map_ne=>?; apply cFunctor_ne.
 Qed.
 Next Obligation.
-  intros C F A B g; simpl. rewrite -{2}(iprod_map_id g).
-  apply iprod_map_ext=> y; apply cFunctor_id.
+  intros C F A B g; simpl. rewrite -{2}(ofe_fun_map_id g).
+  apply ofe_fun_map_ext=> y; apply cFunctor_id.
 Qed.
 Next Obligation.
-  intros C F A1 A2 A3 B1 B2 B3 f1 f2 f1' f2' g. rewrite /= -iprod_map_compose.
-  apply iprod_map_ext=>y; apply cFunctor_compose.
+  intros C F A1 A2 A3 B1 B2 B3 f1 f2 f1' f2' g. rewrite /= -ofe_fun_map_compose.
+  apply ofe_fun_map_ext=>y; apply cFunctor_compose.
 Qed.
 
-Notation "T -c> F" := (@iprodCF T%type (λ _, F%CF)) : cFunctor_scope.
+Notation "T -c> F" := (@ofe_funCF T%type (λ _, F%CF)) : cFunctor_scope.
 
-Instance iprodCF_contractive `{Finite C} (F : C → cFunctor) :
-  (∀ c, cFunctorContractive (F c)) → cFunctorContractive (iprodCF F).
+Instance ofe_funCF_contractive `{Finite C} (F : C → cFunctor) :
+  (∀ c, cFunctorContractive (F c)) → cFunctorContractive (ofe_funCF F).
 Proof.
   intros ? A1 A2 B1 B2 n ?? g.
-  by apply iprodC_map_ne=>c; apply cFunctor_contractive.
+  by apply ofe_funC_map_ne=>c; apply cFunctor_contractive.
 Qed.
 
 (** Constructing isomorphic OFEs *)
